Spqr.lean
@@ -102,6 +102,7 @@ import Spqr.Specs.Chain.EPOCHS_TO_KEEP_PRIOR_TO_SEND_EPOCH
 import Spqr.Specs.Chain.KeyHistory.Add
 import Spqr.Specs.Chain.KeyHistory.Clear
 import Spqr.Specs.Chain.KeyHistory.Gc
+import Spqr.Specs.Chain.KeyHistory.GcLoopPost
 import Spqr.Specs.Chain.KeyHistory.Get
 import Spqr.Specs.Chain.KeyHistory.KEY_SIZE
 import Spqr.Specs.Chain.KeyHistory.New
